

QUBITS AND QUANTUM STATES

December 16, 2025

Exercise 2.1

Given the state:

$$|\psi\rangle = \frac{1-i}{\sqrt{3}}|0\rangle + \frac{1}{\sqrt{3}}|1\rangle$$

The measurement probabilities are:

$$P_0 = \left| \frac{1-i}{\sqrt{3}} \right|^2 = \frac{|1-i|^2}{3} = \frac{2}{3}, \quad P_1 = \left| \frac{1}{\sqrt{3}} \right|^2 = \frac{1}{3}.$$

Checking if probabilities add up to one:

$$P_0 + P_1 = \frac{2}{3} + \frac{1}{3} = 1$$

Exercise 2.2

Let

$$|a\rangle = \begin{pmatrix} -4i \\ 2 \end{pmatrix} \quad |b\rangle = \begin{pmatrix} 1 \\ -1+i \end{pmatrix}.$$

(A) Find $|a+b\rangle$.

$$|a+b\rangle = |a\rangle + |b\rangle = \begin{pmatrix} -4i \\ 2 \end{pmatrix} + \begin{pmatrix} 1 \\ -1+i \end{pmatrix} = \begin{pmatrix} 1-4i \\ 1+i \end{pmatrix}$$

(B) Calculate $3|a\rangle - 2|b\rangle$.

$$3|a\rangle - 2|b\rangle = \begin{pmatrix} -12i \\ 6 \end{pmatrix} + \begin{pmatrix} -2 \\ 2-2i \end{pmatrix} = \begin{pmatrix} -2+8i \\ 8-2i \end{pmatrix}$$

(C) **Normalize** $|a\rangle, |b\rangle$.

$$\langle a|a\rangle = |a\rangle^\dagger * |a\rangle = \begin{pmatrix} 4i & 2 \end{pmatrix} * \begin{pmatrix} -4i \\ 2 \end{pmatrix} = 16 + 4 = 20$$

$$||a|| = \sqrt{\langle a|a\rangle} = \sqrt{20}$$

$$|\tilde{a}\rangle = \frac{|a\rangle}{||a||} = \frac{\begin{pmatrix} -4i \\ 2 \end{pmatrix}}{\sqrt{20}} = \frac{1}{\sqrt{20}} \begin{pmatrix} -4i \\ 2 \end{pmatrix} = \begin{pmatrix} -\frac{2i}{\sqrt{5}} \\ \frac{1}{\sqrt{5}} \end{pmatrix}$$

$$\langle b|b\rangle = |b\rangle^\dagger * |b\rangle = \begin{pmatrix} 1 & -1-i \end{pmatrix} * \begin{pmatrix} 1 \\ -1+i \end{pmatrix} = 1 + 1 + 1 + i - i = 3$$

$$||b|| = \sqrt{\langle b|b\rangle} = \sqrt{3}$$

$$|\tilde{b}\rangle = \frac{|b\rangle}{||b||} = \frac{\begin{pmatrix} 1 \\ -1+i \end{pmatrix}}{\sqrt{3}} = \frac{1}{\sqrt{3}} \begin{pmatrix} 1 \\ -1+i \end{pmatrix} = \begin{pmatrix} \frac{1}{\sqrt{3}} \\ \frac{-1+i}{\sqrt{3}} \end{pmatrix}$$

Exercise 2.3

Another basis for \mathbb{C}^2 Given:

$$|+\rangle = \frac{|0\rangle + |1\rangle}{\sqrt{2}}, |-\rangle = \frac{|0\rangle - |1\rangle}{\sqrt{2}}$$

$$|+\rangle + |-\rangle = \frac{2|0\rangle}{\sqrt{2}} = \sqrt{2}|0\rangle$$

so

$$|0\rangle = \frac{|+\rangle + |-\rangle}{\sqrt{2}}$$

$$|+\rangle - |-\rangle = \frac{2|1\rangle}{\sqrt{2}} = \sqrt{2}|1\rangle$$

so

$$|1\rangle = \frac{|+\rangle - |-\rangle}{\sqrt{2}}$$

These are inverted relations.

Exercise 2.4

a quantum system is in the state

$$|\psi\rangle = \frac{3i|0\rangle + 4|1\rangle}{5}$$

(A) Is the state normalized

To show that it is normalized we must show: $\langle\psi|\psi\rangle = 1$

$$\begin{aligned} |\psi\rangle^\dagger &= -\frac{3i}{5}\langle 0| + \frac{4}{5}\langle 1| \\ \langle\psi|\psi\rangle &= \left(-\frac{3i}{5}\langle 0| + \frac{4}{5}\langle 1|\right) * \left(\frac{3i}{5}|0\rangle + \frac{4}{5}|1\rangle\right) = \\ &= \frac{9}{25}\langle 0|0\rangle + \frac{-12}{25}\langle 0|1\rangle + \frac{12i}{25}\langle 1|0\rangle + \frac{16}{25}\langle 1|1\rangle \end{aligned}$$

Because of the orthonormality relations the only terms left are: $\langle 0|0\rangle = \langle 1|1\rangle = 1$ so

$$\langle\psi|\psi\rangle = \frac{9}{25}\langle 0|0\rangle + \frac{16}{25}\langle 1|1\rangle = \frac{9}{25} + \frac{16}{25} = 1$$

therefore state is normalized

(B) Express the state in the $|+\rangle, |-\rangle$ basis

$$\begin{aligned} |\psi\rangle &= \frac{1}{5}(3i|0\rangle + 4|1\rangle) \Rightarrow |\psi\rangle = \frac{1}{5} \begin{pmatrix} 3i \\ 4 \end{pmatrix} \\ |\psi\rangle &= \frac{1}{5} \begin{bmatrix} 3i \\ 4 \end{bmatrix} = \frac{1}{5} \left[\begin{pmatrix} 3i \\ 0 \end{pmatrix} + \begin{pmatrix} 0 \\ 4 \end{pmatrix} \right] = \frac{1}{5} \left[\frac{1}{2} \begin{pmatrix} 3i + 3i \\ 3i - 3i \end{pmatrix} + \frac{1}{2} \begin{pmatrix} 4 + 4 \\ 4 - 4 \end{pmatrix} \right] = \\ &= \frac{1}{5} \left[\frac{1}{2} \begin{pmatrix} 3i \\ 3i \end{pmatrix} + \frac{1}{2} \begin{pmatrix} 3i \\ -3i \end{pmatrix} + \frac{1}{2} \begin{pmatrix} 4 \\ 4 \end{pmatrix} - \frac{1}{2} \begin{pmatrix} 4 \\ -4 \end{pmatrix} \right] = \\ &= \frac{1}{5} \left[\frac{4 + 3i}{2} \begin{pmatrix} 1 \\ 1 \end{pmatrix} + \frac{-4 + 3i}{2} \begin{pmatrix} 1 \\ -1 \end{pmatrix} \right] = \\ &= \frac{1}{5} \left[\frac{4 + 3i}{\sqrt{2}} \left(\frac{1}{\sqrt{2}} \begin{pmatrix} 1 \\ 1 \end{pmatrix} \right) + \frac{-4 + 3i}{\sqrt{2}} \left(\frac{1}{\sqrt{2}} \begin{pmatrix} 1 \\ -1 \end{pmatrix} \right) \right] = \\ &= \frac{4 + 3i}{5\sqrt{2}} |+\rangle + \frac{-4 + 3i}{5\sqrt{2}} |-\rangle \end{aligned}$$

Exercise 2.5

Gram-Schmidt on \mathbb{R}^4 Given:

$$|u_1\rangle = \begin{pmatrix} 1 \\ 1 \\ 1 \\ 1 \end{pmatrix}, \quad |u_2\rangle = \begin{pmatrix} 1 \\ 2 \\ 4 \\ 5 \end{pmatrix}, \quad |u_3\rangle = \begin{pmatrix} 1 \\ -3 \\ -4 \\ -2 \end{pmatrix},$$

We use tilde to denote normalized vectors

$$|v_1\rangle = |u_1\rangle$$

Norm:

$$\langle u_1 | u_1 \rangle = \begin{pmatrix} 1 & 1 & 1 & 1 \end{pmatrix} * \begin{pmatrix} 1 \\ 1 \\ 1 \\ 1 \end{pmatrix} = 4$$

Normalize:

$$|\tilde{v}_1\rangle = \frac{|v_1\rangle}{\sqrt{\langle u_1 | u_1 \rangle}} = \frac{1}{2} \begin{pmatrix} 1 \\ 1 \\ 1 \\ 1 \end{pmatrix}$$

Second vector:

$$|v_2\rangle = \begin{pmatrix} 1 \\ 2 \\ 4 \\ 5 \end{pmatrix} - \frac{12}{4} \begin{pmatrix} 1 \\ 1 \\ 1 \\ 1 \end{pmatrix} = \begin{pmatrix} -2 \\ -1 \\ 1 \\ 2 \end{pmatrix}$$

Norm:

$$\langle V_2 | V_2 \rangle = \begin{pmatrix} -2 & -1 & 1 & 2 \end{pmatrix} * \begin{pmatrix} -2 \\ -1 \\ 1 \\ 2 \end{pmatrix} = 4 + 1 + 1 + 4 = 10$$

Normalize:

$$|\tilde{v}_2\rangle = \frac{1}{\sqrt{10}} \begin{pmatrix} -2 \\ -1 \\ 1 \\ 2 \end{pmatrix} = \begin{pmatrix} \frac{-2}{\sqrt{10}} \\ \frac{-1}{\sqrt{10}} \\ \frac{1}{\sqrt{10}} \\ \frac{2}{\sqrt{10}} \end{pmatrix}$$

Third vector:

$$|v_3\rangle = \begin{pmatrix} 1 \\ -3 \\ -4 \\ -2 \end{pmatrix} - \frac{-8}{4} \begin{pmatrix} 1 \\ 1 \\ 1 \\ 1 \end{pmatrix} - \frac{-7}{10} \begin{pmatrix} -2 \\ -1 \\ 1 \\ 2 \end{pmatrix} = \begin{pmatrix} \frac{16}{10} \\ \frac{-17}{10} \\ \frac{-13}{10} \\ \frac{14}{10} \end{pmatrix}$$

Norm:

$$\langle V_3|V_3\rangle = \begin{pmatrix} \frac{16}{10} & \frac{-17}{10} & \frac{-13}{10} & \frac{14}{10} \end{pmatrix} * \begin{pmatrix} \frac{16}{10} \\ \frac{-17}{10} \\ \frac{-13}{10} \\ \frac{14}{10} \end{pmatrix} = \frac{910}{100}$$

Normalize:

$$|\tilde{v}_3\rangle = \frac{1}{\sqrt{\frac{910}{100}}} \begin{pmatrix} \frac{16}{10} \\ \frac{-17}{10} \\ \frac{-13}{10} \\ \frac{14}{10} \end{pmatrix} = \frac{10}{\sqrt{910}} \begin{pmatrix} \frac{16}{10} \\ \frac{-17}{10} \\ \frac{-13}{10} \\ \frac{14}{10} \end{pmatrix} = \frac{1}{\sqrt{910}} \begin{pmatrix} 16 \\ -17 \\ -13 \\ 14 \end{pmatrix}$$

The orthonormal basis for the span is:

$$e_1 = \frac{1}{2} \begin{pmatrix} 1 \\ 1 \\ 1 \\ 1 \end{pmatrix} \quad e_2 = \frac{1}{\sqrt{10}} \begin{pmatrix} -2 \\ -1 \\ 1 \\ 2 \end{pmatrix} \quad e_3 = \frac{1}{\sqrt{910}} \begin{pmatrix} 16 \\ -17 \\ -13 \\ 14 \end{pmatrix}$$

Exercise 2.6

Photon horizontal and vertical polarization states are written as $|h\rangle$ and $|v\rangle$ respectively. Suppose:

$$|\psi_1\rangle = \frac{1}{2}|h\rangle + \frac{\sqrt{3}}{2}|v\rangle$$

$$|\psi_2\rangle = \frac{1}{2}|h\rangle - \frac{\sqrt{3}}{2}|v\rangle$$

$$|\psi_3\rangle = |h\rangle$$

$$\langle\psi_1|\psi_2\rangle = (\frac{1}{2}\langle h| + \frac{\sqrt{3}}{2}\langle v|)(\frac{1}{2}|h\rangle - \frac{\sqrt{3}}{2}|v\rangle) = (\frac{1}{2})^2 - (\frac{\sqrt{3}}{2})^2 = -\frac{1}{2}$$

$$|\langle\psi_1|\psi_2\rangle|^2 = (-\frac{1}{2})^2 = \frac{1}{4}$$

$$\langle\psi_1|\psi_3\rangle = (\frac{1}{2}\langle h| + \frac{\sqrt{3}}{2}\langle v|)|h\rangle = \frac{1}{2}$$

$$|\langle\psi_1|\psi_3\rangle|^2 = (\frac{1}{2})^2 = \frac{1}{4}$$

$$\langle\psi_3|\psi_1\rangle = \langle h|(\frac{1}{2}|h\rangle + \frac{\sqrt{3}}{2}|v\rangle) = \frac{1}{2}$$

$$|\langle\psi_3|\psi_1\rangle|^2 = (\frac{1}{2})^2 = \frac{1}{4}$$